(define (A x y)
  (cond ((= y 0) 0)
        ((= x 0) (* 2 y))
        ((= y 1) 2)
        (else (A (- x 1) (A x (- y 1))))))

(A 1 10)
(A 0 (A 1 9))
(* 2 (A 1 9))
= 1024

(A 1 9)
(A 0 (A 1 8))
(* 2 (A 1 8))
= 512

(A 1 8)
(A 0 (A 1 7))
(* 2 (A 1 7))
= 256

(A 1 7)
(A 0 (A 1 6))
(* 2 (A 1 6))
= 128

(A 1 6)
(A 0 (A 1 5))
(* 2 (A 1 5))
= 64

(A 1 5)
(A 0 (A 1 4))
(* 2 (A 1 4))
= 32

(A 1 4)
(A 0 (A 1 3))
(* 2 (A 1 3))
= 16

(A 1 3)
(A 0 (A 1 2))
(* 2 (A 1 2))
= 8

(A 1 2)
(A 0 (A 1 1))
(* 2 (A 1 1))
= 4
---

(A 2 4)
(A 1 (A 2 3))
= (A 1 16) = 65536

(A 2 3)
(A 1 (A 2 2))
= (A 1 4) = 16

(A 2 2)
(A 0 (A 2 1))
(* 2 (A 2 1))
= 4

(A 2 1)
= 2
---

(A 3 3)
(A 2 (A 3 2))
= (A 2 4) = 65536

(A 3 2)
(A 2 (A 3 1))
(A 2 2)
= 4

(define (f n) (A 0 n)) = 2 * n
(define (g n) (A 1 n)) = 2 ^ n
(define (h n) (A 2 n)) = (A 1 (A 2 (n - 1)))
